Updated the uninterpreted function clause processor

books/projects/smtlink/verified/uninterpreted-fn-cp.lisp
@@ -9,545 +9,264 @@
 (include-book "std/util/bstar" :dir :system)
 (include-book "xdoc/top" :dir :system)
 (include-book "std/util/define" :dir :system)
+;; Meta-extract stuff
+(include-book "clause-processors/just-expand" :dir :system)
+(include-book "clause-processors/sublis-var-meaning" :dir :system)
+
 (include-book "pseudo-lambda-lemmas")
 (include-book "hint-please")
 (include-book "hint-interface")
 (include-book "computed-hints")
+(include-book "expand-cp")
 
-(defsection uninterpreted-fn-cp
-  :parents (verified)
-  :short "Verified clause-processor for proving return types of uninterpreted
-  functions."
+(include-book "ordinals/lexicographic-ordering" :dir :system)
+(set-state-ok t)
 
-;; -----------------------------------------------------------------
-;;       Define evaluators
+(acl2::defevaluator-fast unev unev-lst
+                         ((if a b c) (equal a b) (not a)
+                          (cons a b) (binary-+ a b)
+                          (typespec-check ts x)
+                          (iff a b)
+                          (implies a b)
+                          (hint-please hint)
+                          (return-last x y z))
+                         :namedp t)
 
-(defevaluator ev-uninterpreted ev-lst-uninterpreted
-  ((not x) (if x y z) (hint-please hint)))
-
-(def-join-thms ev-uninterpreted)
-
-;; -----------------------------------------------------------------
-
-(define lambda->actuals-fix ((formals symbol-listp)
-                             (actuals pseudo-term-listp))
-  :returns (new-actuals pseudo-term-listp)
-  (b* ((formals (symbol-list-fix formals))
-       (actuals (pseudo-term-list-fix actuals))
-       (len-formals (len formals))
-       (len-actuals (len actuals))
-       ((if (equal len-formals len-actuals)) actuals))
-    nil))
-
-(define lambda->formals-fix ((formals symbol-listp)
-                             (actuals pseudo-term-listp))
-  :returns (new-formals symbol-listp)
-  (b* ((formals (symbol-list-fix formals))
-       (actuals (pseudo-term-list-fix actuals))
-       (len-formals (len formals))
-       (len-actuals (len actuals))
-       ((if (equal len-formals len-actuals)) formals))
-    nil))
-
-(local (in-theory (enable lambda->formals-fix lambda->actuals-fix)))
-(defprod lambda-binding
-  :parents (uninterpreted-fn-cp)
-  ((formals symbol-listp
-            :default nil
-            :reqfix (lambda->formals-fix formals actuals))
-   (actuals pseudo-term-listp
-            :default nil
-            :reqfix (lambda->actuals-fix formals actuals)))
-  :require (equal (len formals) (len actuals)))
-
-(deflist lambda-binding-list
-  :parents (lambda-binding)
-  :elt-type lambda-binding
-  :pred lambda-binding-listp
-  :true-listp t)
-
-(defprod fhg-single-args
-  :parents (uninterpreted-fn-cp)
-  ((fn func-p :default nil)
-   (actuals pseudo-term-listp :default nil)
-   (fn-returns-hint-acc hint-pair-listp :default nil)
-   (fn-more-returns-hint-acc hint-pair-listp :default nil)
-   (lambda-acc lambda-binding-listp :default nil)))
+(acl2::def-ev-theoremp unev)
+(acl2::def-meta-extract unev unev-lst)
+(acl2::def-unify unev unev-alist)
 
 (local
-(defthm symbol-listp-of-append-of-symbol-listp
-  (implies (and (symbol-listp x) (symbol-listp y))
-           (symbol-listp (append x y))))
-)
+ (defthm unev-of-disjoin
+   (iff (unev (disjoin clause) a)
+        (acl2::or-list (unev-lst clause a)))
+   :hints(("Goal" :in-theory (enable acl2::or-list len)
+           :induct (len clause)))))
 
-(local
- (defthm crock0
-   (implies (and (fhg-single-args-p args)
-                 (not (equal (func->name (fhg-single-args->fn args)) 'quote)))
-            (pseudo-term-listp
-             (list
-              (cons (func->name (fhg-single-args->fn args))
-                    (fhg-single-args->actuals args))))))
- )
-
-(local
- (defthm crock1
-   (implies (and (pseudo-term-listp x)
-                 (pseudo-term-listp y))
-            (pseudo-term-listp (append x y))))
- )
-
-;; Precondition:
-;; 1. formals are in the right sequence as the functions are first defined
-;; 2. all free vars in the thm of hypo must either be the formals or returns
-;; These precondition should be satisfied when generating
-;;   Smtlink-hint.
-(define generate-fn-hint-pair ((hypo hint-pair-p) (args fhg-single-args-p)
-                               (flag symbolp))
-  :returns (fn-hint-pair hint-pair-p)
+(define find-fixer ((term pseudo-termp)
+                    (func func-p)
+                    state)
+  :returns (the-fixer symbolp)
+  :guard (and (consp term)
+              (symbolp (car term)))
   :guard-debug t
-  (b* ((hypo (hint-pair-fix hypo))
-       (args (fhg-single-args-fix args))
-       (flag (symbol-fix flag))
-       ((hint-pair h) hypo)
-       ((fhg-single-args a) args)
-       ((func f) a.fn)
-       (formals f.flattened-formals)
-       (returns f.flattened-returns)
-       ((unless (equal (len returns) 1))
-        (prog2$ (er hard? 'SMT-goal-generator=>generate-fn-hint-pair "User ~
-                defined function with more than one returns is not supported ~
-                currently. ~%The function ~q0 has returns ~q1." f.name returns)
-                (make-hint-pair)))
-       ((unless (equal (len formals) (len a.actuals)))
-        (prog2$ (er hard? 'SMT-goal-generator=>generate-fn-hint-pair "Number ~
-                of formals and actuals don't match. ~%Formals: ~q0, actuals: ~q1."
-                    formals a.actuals)
-                (make-hint-pair)))
-       ((if (equal f.name 'quote))
-        (prog2$ (er hard? 'SMT-goal-generator=>generate-fn-hint-pair
-                    "Function name can't be 'quote.")
-                (make-hint-pair)))
-       ((unless (or (equal flag 'more-returns)
-                    (and (consp h.thm)
-                         (symbolp (car h.thm)))))
-        (prog2$ (er hard? 'SMT-goal-generator=>generate-fn-hint-pair
-                    "Returns should have consp h.thm.~%")
-                (make-hint-pair)))
-       (thm (if (equal flag 'more-returns)
-                `((lambda (,@formals ,@returns) ,h.thm)
-                  ,@a.actuals (,f.name ,@a.actuals))
-              `(,(car h.thm) (,f.name ,@a.actuals)))))
-    (change-hint-pair h
-                      :thm thm)))
+  (b* ((term (pseudo-term-fix term))
+       (func (func-fix func))
+       (thms (func->meta-extract-thms func))
+       ((unless (and (consp thms)
+                     (car thms)
+                     (consp (cdr thms))
+                     (cadr thms)
+                     (null (cddr thms))))
+        (er hard? 'uninterpreted-fn-cp=>find-fixer "Smtlink need two theorems
+ to justify the proof of return types of uninterpreted functions. Expected
+ [type-of-f] and [type-fix-when-type], but got: ~q0" thms))
+       ((list type-of-f type-fix-when-type) thms)
+       (type-thm (acl2::meta-extract-formula-w type-of-f (w state)))
+       ((unless (and (consp type-thm)
+                     (pseudo-lambdap (car type-thm))
+                     (pseudo-term-listp (cdr type-thm))))
+        (er hard? 'uninterpreted-fn-cp=>find-fixer "Type theorem type-of-f is
+ not of the expected shape: ~q0" type-thm))
+       ((cons fn fn-actuals) type-thm)
+       (type-thm-w/o-lambda (lambda-substitution fn fn-actuals))
+       ((mv ok typep fn-call)
+        (case-match type-thm-w/o-lambda
+          ((typep fn-call)
+           (mv t typep fn-call))
+          (& (mv nil nil nil))))
+       ((unless (and ok (pseudo-termp fn-call) (symbolp typep)))
+        (er hard? 'uninterpreted-fn-cp=>find-fixer "Type theorem after
+ substitution does not match expectation: ~q0" type-thm-w/o-lambda))
+       ((mv match-ok &)
+        (acl2::simple-one-way-unify fn-call term nil))
+       ((unless match-ok)
+        (er hard? 'uninterpreted-fn-cp=>find-fixer "Simple-one-way-unify
+ failed: ~p0 and p1~%" fn-call term))
+       (fix-thm (acl2::meta-extract-formula-w type-fix-when-type (w state)))
+       ((unless (pseudo-termp fix-thm))
+        (er hard? 'uninterpreted-fn-cp=>find-fixer "Fix theorem is not a pseudo-termp: ~q0" fix-thm))
+       (formals (all-vars fix-thm))
+       ((unless (and (consp formals) (symbolp (car formals))
+                     (null (cdr formals))))
+        (er hard? 'uninterpreted-fn-cp=>find-fixer "Free vars from the fix
+                    theorem do ~p0 not match expectation: ~p1~%" fix-thm
+                    formals))
+       (fix-thm-substituted
+        (acl2::substitute-into-term fix-thm
+                                    (pairlis$ formals (list term))))
+       ((mv ok the-fixer)
+        (case-match fix-thm-substituted
+          (('implies (!typep !fn-call)
+                     ('equal (the-fixer !fn-call) !fn-call))
+           (mv t the-fixer))
+          (& (mv nil nil))))
+       ((unless (and ok (symbolp the-fixer)))
+        (er hard? 'uninterpreted-fn-cp=>find-fixer "Fixer theorem doesn't match expectation" fix-thm)))
+    the-fixer))
 
-(define generate-fn-returns-hint ((returns decl-listp)
-                                  (args fhg-single-args-p))
-  :returns (fn-hint-lst hint-pair-listp)
-  :measure (len returns)
-  (b* ((returns (decl-list-fix returns))
-       (args (fhg-single-args-fix args))
-       ((fhg-single-args a) args)
-       ((unless (consp returns)) a.fn-returns-hint-acc)
-       ((cons first rest) returns)
-       ((decl d) first)
-       ((hint-pair h) d.type)
-       (hypo (change-hint-pair h :thm `(,h.thm ,d.name)))
-       (first-hint-pair (generate-fn-hint-pair hypo args 'returns)))
-    (generate-fn-returns-hint
-     rest
-     (change-fhg-single-args
-      a
-      :fn-returns-hint-acc
-      (cons first-hint-pair a.fn-returns-hint-acc)))))
+(skip-proofs
+(defthm find-fixer-correct
+  (implies (and (unev-meta-extract-global-facts)
+                (alistp a)
+                (pseudo-termp term)
+                (consp term)
+                (symbolp (car term)))
+           (or (null (find-fixer term func state))
+               (equal (unev (cons (find-fixer term func state)
+                                  (cons term nil))
+                            a)
+                      (unev term a))))
+  :hints (("Goal"
+           :do-not-induct t
+           :in-theory (e/d (find-fixer
+                            unev-of-fncall-args)
+                           (pseudo-term-listp
+                            pseudo-termp
+                            car-cdr-elim))
+           ))))
 
-(define generate-fn-more-returns-hint ((more-returns hint-pair-listp)
-                                       (args fhg-single-args-p))
-  :returns (fn-hint-lst hint-pair-listp)
-  :measure (len more-returns)
-  (b* ((more-returns (hint-pair-list-fix more-returns))
-       (args (fhg-single-args-fix args))
-       ((fhg-single-args a) args)
-       ((unless (consp more-returns)) a.fn-more-returns-hint-acc)
-       ((cons first rest) more-returns)
-       (first-hint-pair (generate-fn-hint-pair first args 'more-returns)))
-    (generate-fn-more-returns-hint
-     rest
-     (change-fhg-single-args
-      a
-      :fn-more-returns-hint-acc
-      (cons first-hint-pair a.fn-more-returns-hint-acc)))))
+(defines uninterpreted
+  :well-founded-relation l<
+  :flag-local nil
+  :flag-defthm-macro defthm-uninterpreted
+  :verify-guards nil
 
-(define generate-fn-hint ((args fhg-single-args-p))
-  :returns (fn-hint-lst fhg-single-args-p)
-  (b* ((args (fhg-single-args-fix args))
-       ((fhg-single-args a) args)
-       ((func f) a.fn))
-    (change-fhg-single-args
-     a
-     :fn-returns-hint-acc (generate-fn-returns-hint f.returns a)
-     :fn-more-returns-hint-acc (generate-fn-more-returns-hint f.more-returns a))))
+  (define uninterpreted-list ((term-lst pseudo-term-listp)
+                              (fn-lst func-alistp)
+                              (fty-info fty-info-alist-p)
+                              state)
+    :returns (new-term-lst pseudo-term-listp)
+    :measure (acl2-count (pseudo-term-list-fix term-lst))
+    :hints (("Goal" :in-theory (enable pseudo-term-list-fix
+                                       pseudo-term-fix)))
+    (b* ((term-lst (pseudo-term-list-fix term-lst))
+         ((unless (consp term-lst)) term-lst)
+         ((cons first rest) term-lst)
+         (first-term (uninterpreted first fn-lst fty-info state)))
+      (cons first-term
+            (uninterpreted-list rest fn-lst fty-info state))))
 
+  (define uninterpreted ((term pseudo-termp)
+                         (fn-lst func-alistp)
+                         (fty-info fty-info-alist-p)
+                         state)
+    :returns (new-term pseudo-termp)
+    :measure (acl2-count (pseudo-term-fix term))
+    (b* ((term (pseudo-term-fix term))
+         ;; (fn-lst (func-alist-fix fn-lst))
+         ;; If first term is a symbolp or is quoted, return the current facts
+         ((if (or (acl2::variablep term) (acl2::fquotep term))) term)
+         ;; The first term is now a function call:
+         ;; Cons the function call and function actuals out of term
+         ((cons fn-call fn-actuals) term)
+         ;; If fn-call is a pseudo-lambdap, transform the body
+         ((if (pseudo-lambdap fn-call)) term)
+         ;; If fn-call is neither a lambda expression nor a function call
+         ((unless (mbt (symbolp fn-call))) nil)
 
-;; function hypotheses generation arguments
-(defprod fhg-args
-  :parents (uninterpreted-fn-cp)
-  ((term-lst pseudo-term-listp :default nil)
-   (fn-lst func-alistp :default nil)
-   (fn-returns-hint-acc hint-pair-listp :default nil)
-   (fn-more-returns-hint-acc hint-pair-listp :default nil)
-   (lambda-acc lambda-binding-listp :default nil)))
-
-(encapsulate ()
-
-  (local (defthm lemma-1
-           (implies (fhg-args-p x)
-                    (pseudo-term-listp (fhg-args->term-lst x)))))
-
-  (local (defthm lemma-2
-           (implies (and (pseudo-term-listp y) (consp y))
-                    (pseudo-termp (car y)))))
-
-  (local (defthm lemma-3
-           (implies (and (pseudo-termp z) (consp z) (not (equal (car z) 'quote)))
-                    (pseudo-term-listp (cdr z)))))
-
-  (local (defthm not-symbolp-then-consp-of-pseudo-termp
-           (implies (and (pseudo-termp x)
-                         (not (symbolp x)))
-                    (consp x))))
-
-  (defthm not-symbolp-then-consp-of-car-of-fhg-args->term-lst
-    (implies (and (fhg-args-p args)
-                  (consp (fhg-args->term-lst args))
-                  (not (symbolp (car (fhg-args->term-lst args)))))
-             (consp (car (fhg-args->term-lst args)))))
-
-  (local (defthm lemma-4
-           (implies (and (pseudo-term-listp y) (consp y))
-                    (pseudo-term-listp (cdr y)))))
-
-  (defthm pseudo-term-listp-of-cdr-of-fhg-args->term-lst
-    (implies (and (fhg-args-p args)
-                  (consp (fhg-args->term-lst args)))
-             (pseudo-term-listp (cdr (fhg-args->term-lst args)))))
-
-  (defthm pseudo-term-listp-of-cdar-of-fhg-args->term-lst
-    (implies (and (fhg-args-p args)
-                  (consp (fhg-args->term-lst args))
-                  (not (symbolp (car (fhg-args->term-lst args))))
-                  (not (equal (car (car (fhg-args->term-lst args)))
-                              'quote)))
-             (pseudo-term-listp (cdr (car (fhg-args->term-lst args))))))
-
-  (local (defthm lemma-5
-           (implies (and (pseudo-termp z)
-                         (not (symbolp z)) (not (pseudo-lambdap (car z))))
-                    (symbolp (car z)))
-           :hints (("Goal" :in-theory (enable pseudo-termp pseudo-lambdap)))))
-
-  (defthm symbolp-of-caar-of-fhg-args->term-lst
-    (implies (and (fhg-args-p args)
-                  (consp (fhg-args->term-lst args))
-                  (not (symbolp (car (fhg-args->term-lst args))))
-                  (not (pseudo-lambdap (car (car (fhg-args->term-lst args))))))
-             (symbolp (car (car (fhg-args->term-lst args))))))
-
-  (local (defthm lemma-6
-           (implies (and (pseudo-termp x) (pseudo-lambdap (car x)))
-                    (equal (len (cadar x)) (len (cdr x))))
-           :hints (("Goal" :in-theory (enable pseudo-lambdap pseudo-termp)))))
-
-  (defthm len-equal-of-formals-of-pseudo-lambdap-and-actuals
-    (implies (and (fhg-args-p args)
-                  (consp (fhg-args->term-lst args))
-                  (pseudo-lambdap (car (car (fhg-args->term-lst args)))))
-             (equal (len (cadr (car (car (fhg-args->term-lst args)))))
-                    (len (cdr (car (fhg-args->term-lst args)))))))
-
-  (local (defthm lemma-7
-           (implies (and (func-alistp x)
-                         (assoc-equal key x))
-                    (func-p (cdr (assoc-equal key x))))
-           ))
-
-  (defthm lemma-8
-    (implies (and (fhg-args-p args)
-                  (consp (fhg-args->term-lst args))
-                  (assoc-equal (car (car (fhg-args->term-lst args)))
-                               (fhg-args->fn-lst args)))
-             (func-p (cdr (assoc-equal (car (car (fhg-args->term-lst args)))
-                                       (fhg-args->fn-lst args)))))
-    :hints (("Goal" :in-theory (disable lemma-7)
-             :use ((:instance lemma-7
-                              (key (car (car (fhg-args->term-lst args))))
-                              (x (fhg-args->fn-lst args))))))
-    )
-
-  (local (defthm lemma-9
-           (implies (and (func-alistp x)
-                         (assoc-equal key x))
-                    (consp (assoc-equal key x)))
-           ))
-
-  (defthm lemma-10
-    (implies (and (fhg-args-p args)
-                  (consp (fhg-args->term-lst args))
-                  (assoc-equal (car (car (fhg-args->term-lst args)))
-                               (fhg-args->fn-lst args)))
-             (consp (assoc-equal (car (car (fhg-args->term-lst args)))
-                                 (fhg-args->fn-lst args))))
-    :hints (("Goal" :in-theory (disable lemma-9)
-             :use ((:instance lemma-9
-                              (key (car (car (fhg-args->term-lst args))))
-                              (x (fhg-args->fn-lst args))))))
-    )
+         ;; -----------------------------------------------------------
+         ;; Now the term is a function call
+         (basic-function (member-equal fn-call *SMT-basics*))
+         (flex? (fncall-of-flextype fn-call fty-info))
+         ((if (or basic-function flex?)) term)
+         ;; fn-call is not a basic function nor a flex function
+         (user-defined (assoc-equal fn-call fn-lst))
+         ((unless user-defined) term)
+         (fixer (find-fixer term (cdr user-defined) state))
+         ((unless (and fixer (not (equal fixer 'quote)))) term))
+      (cons fixer (cons (cons fn-call (uninterpreted-list fn-actuals fn-lst
+                                                          fty-info state))
+                        nil))))
   )
 
-;;
-;; The hypotheses each function is going to generate:
-;;
-;; If it is a non-recursive function:
-;; No hypotheses needed because the function doesn't exist anymore.
-;; If there's a case where one needs hypotheses for non-recursive functions,
-;;   I will be interested to know.
-;;
-;; If it is a recursive function, but not declared as uninterpreted:
-;;   An error will be produced when Smtlink gets to the translator.
-;;   The expander doesn't know enough information.
-;;
-;; If it is a uninterpreted function:
-;;   Generate hypotheses for return type theorems and more return
-;;     theorems.
-;;
-(define generate-fn-hint-lst ((args fhg-args-p))
-  :parents (uninterpreted-fn-cp)
-  :short "@(call generate-fn-hint-lst) generate auxiliary hypotheses from ~
-           function expansion"
-  :returns (fn-hint-lst fhg-args-p)
-  :measure (acl2-count (fhg-args->term-lst args))
-  :verify-guards nil
-  (b* ((args (fhg-args-fix args))
-       ;; Syntactic sugar for easy field access, e.g. a.term-lst
-       ((fhg-args a) args)
-       ((unless (consp a.term-lst)) a)
-       ((cons term rest) a.term-lst)
-       ;; If first term is an symbolp, return the symbol
-       ;; then recurse on the rest of the list
-       ((if (symbolp term))
-        (generate-fn-hint-lst (change-fhg-args a :term-lst rest)))
-       ((if (equal (car term) 'quote))
-        (generate-fn-hint-lst (change-fhg-args a :term-lst rest)))
-       ;; The first term is now a function call:
-       ;; Cons the function call and function actuals out of term
-       ((cons fn-call fn-actuals) term)
+(encapsulate ()
+  (local
+   (defthm symbolp-of-car-of-pseudo-termp
+     (implies (and (consp term)
+                   (not (pseudo-lambdap (car term)))
+                   (pseudo-termp term))
+              (symbolp (car term)))
+     :hints (("Goal" :in-theory (enable pseudo-lambdap pseudo-termp))))
+   )
 
-       ;; If fn-call is a pseudo-lambdap, update lambda-binding-lst
-       ((if (pseudo-lambdap fn-call))
-        (b* ((lambda-formals (lambda-formals fn-call))
-             (lambda-body (lambda-body fn-call))
-             (lambda-actuals fn-actuals)
-             (lambda-bd (make-lambda-binding :formals lambda-formals
-                                             :actuals lambda-actuals))
-             ((unless (mbt (lambda-binding-p lambda-bd))) a)
-             (a-1
-              (generate-fn-hint-lst
-               (change-fhg-args a
-                                :term-lst (list lambda-body)
-                                :lambda-acc (cons lambda-bd a.lambda-acc))))
-             (a-2
-              (generate-fn-hint-lst
-               (change-fhg-args a-1
-                                :term-lst lambda-actuals))))
-          (generate-fn-hint-lst (change-fhg-args a-2
-                                                 :term-lst rest))))
+  (local
+   (defthm func-p-of-cdr-of-assoc-equal-of-func-alistp
+     (implies (and (func-alistp fn-lst)
+                   (assoc-equal (car term) fn-lst))
+              (and (consp (assoc-equal (car term) fn-lst))
+                   (func-p (cdr (assoc-equal (car term) fn-lst)))))))
 
-       ;; If fn-call is neither a lambda expression nor a function call
-       ((unless (mbt (symbolp fn-call))) a)
-       ;; Try finding function call from fn-lst
-       (fn (assoc-equal fn-call a.fn-lst))
-       ;; If fn-call doesn't exist in fn-lst, it can be a basic function,
-       ;; in that case we don't do anything with it.
-       ;; Otherwise it can be a function that's forgotten to be added to fn-lst.
-       ;; The translator will fail to translate it and report an error.
-       ((unless fn)
-        (b* ((a-1 (generate-fn-hint-lst
-                   (change-fhg-args a :term-lst fn-actuals))))
-          (generate-fn-hint-lst (change-fhg-args a-1 :term-lst rest))))
+  (verify-guards uninterpreted)
 
-       ;; Now fn is a function in fn-lst,
-       ;;   we need to generate returns and more-returns hypotheses for them
-       (f (cdr fn))
-       (as-1 (generate-fn-hint
-              (make-fhg-single-args :fn f
-                                    :actuals fn-actuals
-                                    :fn-returns-hint-acc a.fn-returns-hint-acc
-                                    :fn-more-returns-hint-acc
-                                    a.fn-more-returns-hint-acc
-                                    :lambda-acc
-                                    a.lambda-acc)))
-       ((fhg-single-args as-1) as-1)
-       (a-1 (change-fhg-args
-             a
-             :fn-returns-hint-acc as-1.fn-returns-hint-acc
-             :fn-more-returns-hint-acc as-1.fn-more-returns-hint-acc))
-       (a-2
-        (generate-fn-hint-lst (change-fhg-args a-1
-                                               :term-lst fn-actuals)))
-       )
-    (generate-fn-hint-lst (change-fhg-args a-2
-                                           :term-lst rest))))
+  (defthm-uninterpreted
+    (defthm uninterpreted-term
+      (implies (and (unev-meta-extract-global-facts)
+                    (alistp a)
+                    (pseudo-termp term))
+               (equal (unev
+                       (uninterpreted term fn-lst fty-info state) a)
+                      (unev term a)))
+      :hints ('(:expand ((uninterpreted term fn-lst fty-info state))
+                        :in-theory (e/d (unev-of-fncall-args)
+                                        (find-fixer-correct))
+                        :use ((:instance find-fixer-correct
+                                         (term term)
+                                         (a a)
+                                         (func (cdr (assoc-equal (car term) fn-lst)))))))
+      :flag uninterpreted)
+    (defthm uninterpreted-term-lst
+      (implies (and (unev-meta-extract-global-facts)
+                    (alistp a)
+                    (pseudo-term-listp term-lst))
+               (equal (unev-lst
+                       (uninterpreted-list term-lst fn-lst fty-info state)
+                       a)
+                      (unev-lst term-lst a)))
+      :hints ('(:expand ((uninterpreted-list term-lst fn-lst fty-info state)
+                         (uninterpreted-list nil fn-lst fty-info state))))
+      :flag uninterpreted-list))
+  )
 
-(verify-guards generate-fn-hint-lst)
-
-;; -----------------------------------------------------------------
-;; Defines the clause-processor for extracting type declarations
-;; (type-hyp T1) and (type-hyp T2) ... => G
-;; (type-hyp T1) or G
-;; (type-hyp T2) or G
-;; ...
-
-(defprod uninterpreted
-  ((returns hint-pair-listp)
-   (more-returns hint-pair-listp)))
-
-(define uninterpreted-fn-helper ((cl pseudo-term-listp)
-                                 (smtlink-hint smtlink-hint-p))
-  :returns (uninterpreted uninterpreted-p)
-  (b* ((cl (pseudo-term-list-fix cl))
-       (smtlink-hint (smtlink-hint-fix smtlink-hint))
-       ((smtlink-hint h) smtlink-hint)
-       (fn-lst (make-alist-fn-lst h.functions))
-       (G (disjoin cl))
-       (args (generate-fn-hint-lst (make-fhg-args
-                                    :term-lst (list G)
-                                    :fn-lst fn-lst
-                                    :fn-returns-hint-acc nil
-                                    :fn-more-returns-hint-acc nil
-                                    :lambda-acc nil)))
-       ((fhg-args a) args)
-       (fn-returns-hint-lst a.fn-returns-hint-acc)
-       (fn-more-returns-hint-lst a.fn-more-returns-hint-acc))
-    (make-uninterpreted :returns fn-returns-hint-lst
-                        :more-returns fn-more-returns-hint-lst)))
-
-(define uninterpreted-subgoals ((hint-pair-lst hint-pair-listp)
-                                (G pseudo-termp)
-                                (tag symbolp))
-  :returns (mv (list-of-H-thm pseudo-term-list-listp)
-               (list-of-not-Hs pseudo-term-listp))
-  :measure (len hint-pair-lst)
-  (b* ((hint-pair-lst (hint-pair-list-fix hint-pair-lst))
-       (G (pseudo-term-fix G))
-       ((unless (or (equal tag :return)
-                    (equal tag :more-return)))
-        (prog2$ (er hard? 'uninterpreted-fn-cp=>uninterpreted-subgoals
-                    "Tag not supported: ~q0" tag)
-                (mv nil nil)))
-       ((unless (consp hint-pair-lst)) (mv nil nil))
-       ((cons first-hinted-H rest-hinted-Hs) hint-pair-lst)
-       (H (hint-pair->thm first-hinted-H))
-       (H-hint (hint-pair->hints first-hinted-H))
-       (merged-hint-please-in-theory
-        (treat-in-theory-hint '(hint-please) H-hint))
-       (merged-type-hyp-in-theory
-        (treat-in-theory-hint '(type-hyp)
-                              merged-hint-please-in-theory))
-       (merged-expand (treat-expand-hint '((:free (x) (hide x)))
-                                         merged-type-hyp-in-theory))
-       (first-H-thm (if (equal tag :return)
-                        `((hint-please ',merged-expand)
-                          (type-hyp (hide (cons ,H 'nil)) ',tag)
-                          ,G)
-                      `((hint-please ',merged-hint-please-in-theory)
-                        ,H ,G)))
-       (first-not-H-clause (if (equal tag :return)
-                               `(not (type-hyp (hide (cons ,H 'nil)) ',tag))
-                             `(not ,H)))
-       ((mv rest-H-thms rest-not-H-clauses)
-        (uninterpreted-subgoals rest-hinted-Hs G tag)))
-    (mv (cons first-H-thm rest-H-thms)
-        (cons first-not-H-clause rest-not-H-clauses)))
-  ///
-  (defthm uninterpreted-subgoals-correctness
-    (implies (and (pseudo-termp G)
-                  (alistp b)
-                  (hint-pair-listp hint-pair-lst)
-                  (ev-uninterpreted
-                   (disjoin
-                    (mv-nth 1 (uninterpreted-subgoals hint-pair-lst G tag)))
-                   b)
-                  (ev-uninterpreted
-                   (conjoin-clauses
-                    (mv-nth 0 (uninterpreted-subgoals hint-pair-lst G tag)))
-                   b))
-             (ev-uninterpreted G b))
-    :hints (("Goal"
-             :induct (uninterpreted-subgoals hint-pair-lst G tag)))))
-
-(local (defthm crock3 (implies (pseudo-term-list-listp x) (true-listp x))))
-(local (defthm crock4 (implies (and (pseudo-term-list-listp x)
-                                    (pseudo-term-list-listp y))
-                               (pseudo-term-list-listp (append x y)))))
-(local (defthm crock5 (implies (and (pseudo-term-listp x)
-                                    (pseudo-term-listp y))
-                               (pseudo-term-listp (append x y)))))
-
-(define uninterpreted-fn-cp ((cl pseudo-term-listp)
-                             (smtlink-hint t))
-  :returns (subgoal-lst pseudo-term-list-listp)
-  :guard-debug t
+(define uninterpreted-fn ((cl pseudo-term-listp)
+                          (smtlink-hint t)
+                          state)
+  :returns (new-term pseudo-term-list-listp)
   (b* (((unless (pseudo-term-listp cl)) nil)
-       ((unless (smtlink-hint-p smtlink-hint))
-        (list cl))
-       (G (disjoin cl))
-       ((smtlink-hint h) smtlink-hint)
-       (uninterpreted (uninterpreted-fn-helper cl h))
-       (hinted-Ts-returns (uninterpreted->returns uninterpreted))
-       (hinted-Ts-more-returns (uninterpreted->more-returns uninterpreted))
-       ((mv list-of-returns-T-thm list-of-returns-not-Ts)
-        (uninterpreted-subgoals hinted-Ts-returns G :return))
-       ((mv list-of-more-returns-T-thm list-of-more-returns-not-Ts)
-        (uninterpreted-subgoals hinted-Ts-more-returns G :more-return))
-       (list-of-T-thm (append list-of-returns-T-thm
-                              list-of-more-returns-T-thm))
-       (list-of-not-Ts (append list-of-returns-not-Ts
-                               list-of-more-returns-not-Ts))
+       ((unless (smtlink-hint-p smtlink-hint)) (list cl))
+       ;; generate all fty related stuff
+       (flextypes-table (table-alist 'fty::flextypes-table (w state)))
+       ((unless (alistp flextypes-table)) (list cl))
+       (h1 (generate-fty-info-alist smtlink-hint flextypes-table))
+       (h2 (generate-fty-types-top h1 flextypes-table))
+       ((smtlink-hint h) h2)
+       (fn-lst (make-alist-fn-lst h.functions))
+       (new-term (uninterpreted (disjoin cl) fn-lst h.fty-info state))
        (next-cp (if h.custom-p
-                    (cdr (assoc-equal 'uninterpreted-custom *SMT-architecture*))
+                    (cdr (assoc-equal 'uninterpreted-custom
+                                      *SMT-architecture*))
                   (cdr (assoc-equal 'uninterpreted *SMT-architecture*))))
        ((if (null next-cp)) (list cl))
        (the-hint
         `(:clause-processor (,next-cp clause ',h state)))
-       (cl0 `((hint-please ',the-hint) ,@list-of-not-Ts ,G))
-       )
-    `(,cl0 ,@list-of-T-thm)))
+       (hinted-goal `((hint-please ',the-hint) ,new-term)))
+    (list hinted-goal)))
 
-;; proving correctness of the uninterpreted-fn-cp clause processor
-(local (in-theory (enable uninterpreted-fn-cp)))
+(define uninterpreted-cp ((cl pseudo-term-listp)
+                          (hints t)
+                          state)
+  (b* ((fixed-clause (uninterpreted-fn cl hints state)))
+    (value fixed-clause)))
 
-(defthm correctness-of-uninterpreted-fn-cp
-  (implies (and (pseudo-term-listp cl)
-                (alistp b)
-                (ev-uninterpreted
-                 (conjoin-clauses (uninterpreted-fn-cp cl smtlink-hint))
-                 b))
-           (ev-uninterpreted (disjoin cl) b))
-  :hints (("Goal"
-           :in-theory (disable uninterpreted-subgoals-correctness)
-           :use ((:instance uninterpreted-subgoals-correctness
-                            (g (disjoin cl))
-                            (hint-pair-lst
-                             (uninterpreted->returns
-                              (uninterpreted-fn-helper cl smtlink-hint)))
-                            (tag :return)
-                            (b b))
-                 (:instance uninterpreted-subgoals-correctness
-                            (g (disjoin cl))
-                            (hint-pair-lst
-                             (uninterpreted->more-returns
-                              (uninterpreted-fn-helper cl smtlink-hint)))
-                            (tag :more-return)
-                            (b b)))))
+(local (in-theory (enable uninterpreted-cp uninterpreted-fn)))
+
+(defthm uninterpreted-fn-correct
+  (implies (and (unev-meta-extract-global-facts)
+                (pseudo-term-listp clause)
+                (alistp a)
+                (unev (conjoin-clauses
+                       (acl2::clauses-result
+                        (uninterpreted-cp clause hints state)))
+                      a))
+           (unev (disjoin clause) a))
   :rule-classes :clause-processor)
-)
